5.1 done

src/5.t.lean
@@ -29,4 +29,57 @@ deriving Repr
 #check Option Empty
 #check @Option.some Empty
 
-example (x : X)
+
+inductive BOption (α : Type) : Type
+| none : BOption α
+| some : α -> BOption α
+
+instance : Monad BOption where
+  pure arg := BOption.some arg
+  bind _ _ := BOption.none
+
+def monadContract (m : Type → Type) (α β : Type) [Monad m] : Prop :=
+-- pure should be a left identity of bind
+(∀(f : α → m β) (v : α), bind (pure v) f = f v) ∧ 
+--pure should be a right identity of bind
+(∀(v : m α), bind v pure = v) ∧
+--bind should be associative
+(∀(v : m α) (f : α → m β) (g : β → m α), 
+  bind (bind v f) g = bind v (fun x => bind (f x) g))
+
+#check BOption Empty
+#check @BOption.some Empty
+#check @Empty.rec
+
+example : monadContract BOption Empty β := by{
+  unhygienic
+  rw [monadContract];
+  apply And.intro;{
+    intros f v;
+    rw [pure, Applicative.toPure, Monad.toApplicative, instMonadBOption]
+    simp
+    rw [bind, Monad.toBind]
+    simp
+    --follows from empty type
+    trivial
+  }
+  apply And.intro;
+  {
+    intros v;
+    rw [pure, Applicative.toPure, Monad.toApplicative, instMonadBOption]
+    simp
+    rw [bind, Monad.toBind]
+    simp
+    --v can only be BOption.none
+    cases v;
+    --follows from empty type
+    simp [Empty.rec]
+    trivial;
+  }
+  {
+    intros v f g;
+    rw [bind, Monad.toBind, instMonadBOption];
+  }
+}
+
+--example: ∀ (φ : Prop) (x : Empty), ¬φ ∧ φ := by apply Empty.rec 
